Weidenbach_Book/Watched_Literals_Watch_List_Domain.thy
@@ -107,6 +107,15 @@ lemma literals_are_in_\<L>\<^sub>i\<^sub>n_trail_in_lits_of_l:
   \<open>literals_are_in_\<L>\<^sub>i\<^sub>n_trail M \<Longrightarrow> a \<in> lits_of_l M \<Longrightarrow> a \<in># \<L>\<^sub>a\<^sub>l\<^sub>l\<close>
   by (auto simp: literals_are_in_\<L>\<^sub>i\<^sub>n_trail_def lits_of_def)
 
+lemma literals_are_in_\<L>\<^sub>i\<^sub>n_trail_uminus_in_lits_of_l:
+  \<open>literals_are_in_\<L>\<^sub>i\<^sub>n_trail M \<Longrightarrow> -a \<in> lits_of_l M \<Longrightarrow> a \<in># \<L>\<^sub>a\<^sub>l\<^sub>l\<close>
+  by (auto simp: literals_are_in_\<L>\<^sub>i\<^sub>n_trail_def lits_of_def uminus_lit_swap uminus_\<A>\<^sub>i\<^sub>n_iff)
+
+lemma literals_are_in_\<L>\<^sub>i\<^sub>n_trail_uminus_in_lits_of_l_atms:
+  \<open>literals_are_in_\<L>\<^sub>i\<^sub>n_trail M \<Longrightarrow> -a \<in> lits_of_l M \<Longrightarrow> atm_of a \<in># \<A>\<^sub>i\<^sub>n\<close>
+  using literals_are_in_\<L>\<^sub>i\<^sub>n_trail_uminus_in_lits_of_l[of M a]
+  unfolding in_\<L>\<^sub>a\<^sub>l\<^sub>l_atm_of_in_atms_of_iff[symmetric] atms_of_\<L>\<^sub>a\<^sub>l\<^sub>l_\<A>\<^sub>i\<^sub>n[symmetric]
+  .
 end
 
 
